Incorporated mod from J (with further mods to some books) for untranslating car-cdr nests.
Quoting :doc note-7-0:

  Nests of [car] and [cdr] calls are now printed (``untranslated'')
  differently. The old method availed itself of all 28 of the car-cdr
  macros. The new method only introduces 6 of them: cadr, caddr,
  cadddr, cddr, cdddr, cddddr. This code never introduces such macros
  as caar or cddaar, preferring cars and cdrs when necessary. Lisp
  programmers tend to recognize cadr, caddr, and cadddr as the
  accessors for the 1st, 2nd, and 3rd (0-based) elements of a list.
  See community book books/system/untranslate-car-cdr.lisp for
  further discussion and a correctness proof.

proof-checker-b.lisp
@@ -1534,6 +1534,44 @@
          (car alist))
         (t (rassoc-eq-as-car key (cdr alist)))))
 
+(defconst *ca<d^n>r-alist*
+
+; This alist can be constructed as follows in raw Lisp.  Thus, it associates
+; each legal cd..dr macro with the number of ds in its name.
+
+; ? (loop for x in
+; '(cadr           cdar          caar          cddr
+;   caadr   cdadr  cadar  cddar  caaar  cdaar  caddr  cdddr
+;   caaadr  cadadr caadar caddar
+;   cdaadr  cddadr cdadar cdddar
+;                                caaaar cadaar caaddr cadddr
+;                                cdaaar cddaar cdaddr cddddr)
+; collect (cons x (- (length (symbol-name x)) 2)))
+
+  '((CADR . 2) (CDAR . 2) (CAAR . 2) (CDDR . 2)
+    (CAADR . 3) (CDADR . 3) (CADAR . 3) (CDDAR . 3)
+    (CAAAR . 3) (CDAAR . 3) (CADDR . 3) (CDDDR . 3)
+    (CAAADR . 4) (CADADR . 4) (CAADAR . 4) (CADDAR . 4)
+    (CDAADR . 4) (CDDADR . 4) (CDADAR . 4) (CDDDAR . 4)
+    (CAAAAR . 4) (CADAAR . 4) (CAADDR . 4) (CADDDR . 4)
+    (CDAAAR . 4) (CDDAAR . 4) (CDADDR . 4) (CDDDDR . 4)))
+
+(defun car/cdr^n (n term)
+
+; This function assumes that term is a nest of n or more nested calls of car
+; and/or cdr, and returns the term obtained by stripping n such calls.
+
+  (cond
+   ((zp n) term)
+   ((or (variablep term)
+;       (fquotep term)
+        (not (member-eq (car term) '(car cdr))))
+    (er hard 'car/cdr^n
+        "Illegal call: ~x0.~|If you encountered this call in the ~
+         proof-checker, please contact the ACL2 implemntors."
+        `(car/cdr^n ,n ,term)))
+   (t (car/cdr^n (1- n) (fargn term 1)))))
+
 (defun expand-address (addr raw-term term abbreviations iff-flg
                             accumulated-addr-r wrld)
 
@@ -1884,17 +1922,16 @@
                ((implies iff)
                 (expand-address-recurse :new-iff-flg t))
                (t
-                (mv-let
-                 (fn guts)
-                 (car-cdr-nest term)
-                 (cond
-                  (fn
-                   (expand-address-recurse
-                    :ans (append (make-list (- (length (symbol-name fn)) 2)
-                                            :initial-element 1)
-                                 rest-addr)
-                    :new-term guts))
-                  (t (expand-address-recurse))))))))))))
+                (let ((pair (and (consp raw-term)
+                                 (assoc-eq (car raw-term) *ca<d^n>r-alist*))))
+                  (cond
+                   (pair
+                    (expand-address-recurse
+                     :ans (append (make-list (cdr pair)
+                                             :initial-element 1)
+                                  rest-addr)
+                     :new-term (car/cdr^n (cdr pair) term)))
+                   (t (expand-address-recurse))))))))))))
 
 (defmacro dv-error (str alist)
   `(pprogn (print-no-change
