books/system/top.lisp
@@ -6,16 +6,23 @@
 ; functions.  Add an include-book for each new such book.  (Various people have
 ; done so since this book was originally added.)
 
+; See *system-verify-guards-alist* in ACL2 source file boot-strap-pass-2.lisp
+; for how this book relates to which functions in the ACL2 system come up in
+; :logic mode.
+
 (in-package "ACL2")
 
 (include-book "hl-addr-combine")
 (include-book "extend-pathname")
-; The following is not needed in support of ACL2_DEVEL builds, the ACL2
-; devel-check `make' target, or the ACL2 constant *system-verify-guards-alist*.
-; If we uncomment it, then this book depends ultimately on many other books,
-; and certification fails for some of those books for ACL2 built with
-; ACL2_DEVEL set.
+
+; The following (commented-out) form is not needed in support of ACL2_DEVEL
+; builds, the ACL2 devel-check `make' target, or the ACL2 constant
+; *system-verify-guards-alist*.  If we uncomment it, then this book depends
+; ultimately on many other books, and certification fails for some of those
+; books for ACL2 built with ACL2_DEVEL set.
+
 ; (include-book "too-many-ifs")
+
 (include-book "verified-termination-and-guards")
 (include-book "sublis-var")
 (include-book "subcor-var")
@@ -25,3 +32,10 @@
 (include-book "gather-dcls")
 (include-book "meta-extract")
 (include-book "legal-variablep")
+
+; The following is commented out only because we aren't currently motivated to
+; its functions in ACL2 system constant *system-verify-guards-alist*.  Perhaps
+; that would be easy to do, but note that guards would need to be verified for
+; functions defined in untranslate-car-cdr.lisp.
+
+; (include-book "untranslate-car-cdr")
