books/system/untranslate-car-cdr.lisp
@@ -1,0 +1,546 @@
+; Copyright (C) 2014, Regents of the University of Texas
+; Written by J Strother Moore, October, 2014
+; License: A 3-clause BSD license.  See the LICENSE file distributed with ACL2.
+
+; To recertify:
+; (certify-book "untranslate-car-cdr")
+
+; Proof of the Correctness of CADR Centric Untranslation 
+; J Strother Moore
+; Georgetown, TX, October, 2014
+
+; Abstract
+
+; When ACL2 displays a formula to the user, it ``untranslates'' formal
+; (internal-form) terms into terms involving macros.  For example, (CAR (CDR
+; X)) is displayed as (CADR X).  Common Lisp provides 28 macros for the
+; combinations of CARs and CDRs up to four deep.  Given all these available
+; abbreviations how should (CAR (CDR (CDR (CAR (CDR X))))) be displayed?  
+
+; For the first 25 years of ACL2's history, the term above was displayed as
+; (CADDAR (CDR X)).
+
+; The code verified here displays it as (CADDR (CADR X)).
+
+; The old method availed itself of all 28 of the car-cdr macros.  The new
+; method only introduces 6 of them: CADR, CADDR, CADDDR, CDDR, CDDDR, CDDDDR.
+; This code never introduces such macros as CAAR or CDDAAR, preferring CARs and
+; CDRs when necessary.  Lisp programmers tend to recognize CADR, CADDR, and
+; CADDDR as the accessors for the 1st, 2nd, and 3rd (0-based) elements of a
+; list.
+
+; We call this style of untranslation ``CADR Centric'' because it emphasizes
+; the most common use of the car-cdr macros: accessing particular elements of
+; linear lists.
+
+; Perhaps the most important advantage of CADR Centric untranslation is that it
+; operates from the inside out, where the old method operated from the outside
+; in.  The inside out approach is more likely to give related elements related
+; names.  For example, consider the formula
+
+; (p (car (cdr (car (cdr x))))
+;    (car (cdr (cdr (car (cdr x))))))
+
+; In the old style this would be displayed as
+
+; (p (cadadr x)
+;    (caddar (cdr x)))
+
+; whereas in the new style it is displayed as
+
+; (p (cadr (cadr x))
+;    (caddr (cadr x)))
+
+; which makes it clear that p is being applied to the 1st and 2nd elements of
+; the 1st element of x.
+
+; Because I found the code confusing, I decided to prove that the untranslation
+; preserved the meaning of the original term.  The main theorem proved at the
+; bottom of this book is:
+
+; (DEFTHM UNTRANSLATE-CAR-CDR-NEST-CORRECT
+;   (EQUAL (EVAD TERM ALIST)
+;          (EVAD (UNTRANSLATE-CAR-CDR-NEST TERM) ALIST))
+;   :RULE-CLASSES NIL)
+
+; where evad is an ACL2 evaluator that can handle CAR, CDR, and the six macros
+; possibly introduced by CADR Centric untranslation.  Note that evad cannot be
+; introduced by defevaluator because that event only allows function symbols to
+; be interpreted, whereas CADR, CDDR, etc., are macro symbols.  But the
+; constraints on evad are exactly analogous to what defevaluator generates.
+; For example, 
+
+; (DEFTHM EVAD-CONSTRAINT-10
+;   (IMPLIES (AND (CONSP X) (EQUAL (CAR X) 'CADDR))
+;            (EQUAL (EVAD X A)
+;                   (CADDR (EVAD (CADR X) A)))))
+
+; Note also that UNTRANSLATE-CAR-CDR-NEST-CORRECT does not establish that
+; untranslate-car-cdr-nest returns a well-formed term.
+
+; The problem with well-formedness in this context is that there are two senses
+; of that word: well-formed before untranslation and well-formed after
+; untranslation.  In practice in the ACL2 system, the input to untranslation is
+; a formal (``translated'') ACL2 term: no macros are used.  The output is
+; ``well-formed'' in a different sense, meaning that the macros introduced
+; expand without error.  For example, ACL2's untranslator may see
+; (IF a b (IF c d e)) as input and return (COND (a b) (c d) (T e)) as
+; input and they are well-formed in different senses.
+
+; The function untranslate-car-cdr-nest verified here operates in two phases.
+; Phase 1 extracts a list of As and Ds corresponding to the cAr and cDr symbols
+; surrounding some base.  Phase 1 returns the list and the base.  Phase 2 then
+; wraps a nest of the CADR Centric functions and macros around the base.  But
+; when this code is used by ACL2's full untranslate mechanism, a recursive call
+; of ACL2's mechanism is interposed on the base between phases 1 and 2.  Thus,
+; the base identified by phase 1 is in translated form but the term supplied to
+; phase 2 is in untranslated form.  Thus, the senses in which the inputs to
+; phases 1 and 2 are well-formed are different.
+
+; But in this book, we ignore ACL2's full untranslation mechanism.  We just
+; compose phases 1 and 2, make no assumptions about the shapes of the terms
+; being manipulated, and just prove that the input and output have the same
+; meaning in the EVAD sense.
+
+; -----------------------------------------------------------------
+; Implementation: This single page contains the implementation (and its
+; termination proof).  The rest of this ridiculously long file is the
+; specification and proof of correctness!
+
+(in-package "ACL2")
+
+(program)
+
+(defun make-reversed-ad-list (term ans)
+
+; We treat term as a CAR/CDR nest around some ``base'' and return (mv ad-lst
+; base), where ad-lst is the reversed list of #\A and #\D characters and base
+; is the base of the CAR/CDR nest.  Thus, (CADDR B) into (mv '(#\D #\D #\A) B).
+; If term is not a CAR/CDR nest, adr-lst is nil.
+
+  (cond ((variablep term)
+         (mv ans term))
+        ((fquotep term)
+         (mv ans term))
+        ((eq (ffn-symb term) 'CAR)
+         (make-reversed-ad-list (fargn term 1) (cons '#\A ans)))
+        ((eq (ffn-symb term) 'CDR)
+         (make-reversed-ad-list (fargn term 1) (cons '#\D ans)))
+        (t (mv ans term))))
+
+(defun car-cdr-abbrev-name (adr-lst)
+; Given an adr-lst we turn it into one of the CAR/CDR abbreviation names.  We
+; assume the adr-lst corresponds to a legal name, e.g., its length is no
+; greater than five (counting the #\R).
+  (intern (coerce (cons #\C adr-lst) 'string) "ACL2"))
+
+(defun pretty-parse-ad-list (ad-list dr-list n base)
+  (cond
+   ((eql n 5)
+    (pretty-parse-ad-list ad-list '(#\R) 1
+                          (list (car-cdr-abbrev-name dr-list) base)))
+   ((endp ad-list)
+    (cond ((eql n 1) base)
+          (t (list (car-cdr-abbrev-name dr-list) base))))
+   ((eql (car ad-list) #\A)
+    (pretty-parse-ad-list (cdr ad-list) '(#\R) 1
+                          (list (car-cdr-abbrev-name (cons #\A dr-list)) base)))
+   (t ; (eql (car ad-list) '#\D)
+    (pretty-parse-ad-list (cdr ad-list) (cons #\D dr-list) (+ 1 n) base))))
+
+(defun untranslate-car-cdr-nest (term)
+
+; Examples:
+; (untranslate-car-cdr-nest '(car (cdr (car b))))
+; ==> (CADR (CAR B))
+; (untranslate-car-cdr-nest '(car (cdr (cdr b))))
+; ==> (CADDR B)
+; (untranslate-car-cdr-nest '(car (car (cdr (cdr b)))))
+; ==> (CAR (CADDR B))
+
+  (mv-let (ad-list base)
+          (make-reversed-ad-list term nil)
+          (cond
+           ((null ad-list) base)
+           (t (pretty-parse-ad-list ad-list '(#\R) 1 base)))))
+
+; -----------------------------------------------------------------
+; Conversion to Logic Mode
+
+(logic)
+(include-book "ordinals/lexicographic-ordering" :dir :system)
+
+(verify-termination make-reversed-ad-list)
+(verify-termination car-cdr-abbrev-name)
+(verify-termination pretty-parse-ad-list
+ (declare (xargs :measure (llist (acl2-count ad-list) (nfix n))
+                 :well-founded-relation l<)))
+(verify-termination untranslate-car-cdr-nest)
+
+; -----------------------------------------------------------------
+; Specification Related Functions and Simple Theorems about Them
+
+; There are three types of lists of interest here: lists of #\As and #\Ds,
+; lists of #\Ds with last element #\R, and list of that second type optionally
+; extended with a single #\A.  We call these ``AD'', ``DR'', and ``ADR'' lists,
+; respectively.
+
+(defun ad-listp (x)
+  (cond ((endp x) (eq x nil))
+        ((eql (car x) #\A) (ad-listp (cdr x)))
+        ((eql (car x) #\D) (ad-listp (cdr x)))
+        (t nil)))
+
+(defun dr-listp (x)
+  (cond ((endp x) nil)
+        ((eql (car x) #\R) (equal (cdr x) nil))
+        ((eql (car x) #\D) (dr-listp (cdr x)))
+        (t nil)))
+
+(defun adr-listp (x)
+  (cond ((endp x) nil)
+        ((eql (car x) #\A)
+         (dr-listp (cdr x)))
+        (t (dr-listp x))))
+
+(defun compose-ad (ad-list term)
+
+; We treat ad-list as a list of #\A and #\D, ignoring all other elements.  This
+; allows us to call it on lists of #\D terminated by #\R, which is another
+; ``data type'' in this system.
+
+  (cond ((endp ad-list) term)
+        ((eql (car ad-list) #\A)
+         (compose-ad (cdr ad-list) (list 'CAR term)))
+        ((eql (car ad-list) #\D)
+         (compose-ad (cdr ad-list) (list 'CDR term)))
+        (t (compose-ad (cdr ad-list) term))))
+
+; Imagine we allowed macros to be ``function symbols'' in defevaluator.
+; Then this form:
+
+; (defevaluator evad evad-lst
+;   ((CAR x)
+;    (CDR x)
+;    (CADR x)
+;    (CDDR x)
+;    (CADDR x)
+;    (CDDDR x)
+;    (CADDDR x)
+;    (CDDDDR x)))
+
+; would expand to:
+
+(encapsulate
+ (((evad * *) => *)
+  ((evad-lst * *) => *))
+ (set-inhibit-warnings "theory")
+ (local (in-theory *defevaluator-form-base-theory*))
+ (local (mutual-recursion
+         (defun-nx evad (x a)
+           (declare (xargs :verify-guards nil
+                           :measure (acl2-count x)
+                           :well-founded-relation o<
+                           :mode :logic))
+           (cond ((symbolp x)
+                  (and x (cdr (assoc-eq x a))))
+                 ((atom x) nil)
+                 ((eq (car x) 'quote) (car (cdr x)))
+                 ((consp (car x))
+                  (evad (car (cdr (cdr (car x))))
+                        (pairlis$ (car (cdr (car x)))
+                                  (evad-lst (cdr x) a))))
+                 ((equal (car x) 'car)
+                  (car (evad (car (cdr x)) a)))
+                 ((equal (car x) 'cdr)
+                  (cdr (evad (car (cdr x)) a)))
+                 ((equal (car x) 'cadr)
+                  (cadr (evad (car (cdr x)) a)))
+                 ((equal (car x) 'cddr)
+                  (cddr (evad (car (cdr x)) a)))
+                 ((equal (car x) 'caddr)
+                  (caddr (evad (car (cdr x)) a)))
+                 ((equal (car x) 'cdddr)
+                  (cdddr (evad (car (cdr x)) a)))
+                 ((equal (car x) 'cadddr)
+                  (cadddr (evad (car (cdr x)) a)))
+                 ((equal (car x) 'cddddr)
+                  (cddddr (evad (car (cdr x)) a)))
+                 (t nil)))
+         (defun-nx evad-lst (x-lst a)
+           (declare (xargs :measure (acl2-count x-lst)
+                           :well-founded-relation o<))
+           (cond ((endp x-lst) nil)
+                 (t (cons (evad (car x-lst) a)
+                          (evad-lst (cdr x-lst) a)))))))
+ (local (defthm eval-list-kwote-lst
+          (equal (evad-lst (kwote-lst args) a)
+                 (fix-true-list args))))
+ (defthmd
+   evad-constraint-0
+   (implies (and (consp x)
+                 (syntaxp (not (equal a ''nil)))
+                 (not (equal (car x) 'quote)))
+            (equal (evad x a)
+                   (evad (cons (car x)
+                               (kwote-lst (evad-lst (cdr x) a)))
+                         nil)))
+   :hints
+   (("Goal" :expand ((:free (x) (hide x)) (evad x a))
+     :in-theory (disable (:executable-counterpart evad)))))
+ (defthm evad-constraint-1
+   (implies (symbolp x)
+            (equal (evad x a)
+                   (and x (cdr (assoc-equal x a))))))
+ (defthm evad-constraint-2
+   (implies (and (consp x) (equal (car x) 'quote))
+            (equal (evad x a) (cadr x))))
+ (defthm evad-constraint-3
+   (implies (and (consp x) (consp (car x)))
+            (equal (evad x a)
+                   (evad (caddar x)
+                         (pairlis$ (cadar x)
+                                   (evad-lst (cdr x) a))))))
+ (defthm evad-constraint-4
+   (implies (not (consp x-lst))
+            (equal (evad-lst x-lst a) nil)))
+ (defthm evad-constraint-5
+   (implies (consp x-lst)
+            (equal (evad-lst x-lst a)
+                   (cons (evad (car x-lst) a)
+                         (evad-lst (cdr x-lst) a)))))
+ (defthm evad-constraint-6
+   (implies (and (consp x) (equal (car x) 'car))
+            (equal (evad x a)
+                   (car (evad (cadr x) a)))))
+ (defthm evad-constraint-7
+   (implies (and (consp x) (equal (car x) 'cdr))
+            (equal (evad x a)
+                   (cdr (evad (cadr x) a)))))
+ (defthm evad-constraint-8
+   (implies (and (consp x) (equal (car x) 'cadr))
+            (equal (evad x a)
+                   (cadr (evad (cadr x) a)))))
+ (defthm evad-constraint-9
+   (implies (and (consp x) (equal (car x) 'cddr))
+            (equal (evad x a)
+                   (cddr (evad (cadr x) a)))))
+ (defthm evad-constraint-10
+   (implies (and (consp x) (equal (car x) 'caddr))
+            (equal (evad x a)
+                   (caddr (evad (cadr x) a)))))
+ (defthm evad-constraint-11
+   (implies (and (consp x) (equal (car x) 'cdddr))
+            (equal (evad x a)
+                   (cdddr (evad (cadr x) a)))))
+ (defthm evad-constraint-12
+   (implies (and (consp x) (equal (car x) 'cadddr))
+            (equal (evad x a)
+                   (cadddr (evad (cadr x) a)))))
+ (defthm evad-constraint-13
+   (implies (and (consp x) (equal (car x) 'cddddr))
+            (equal (evad x a)
+                   (cddddr (evad (cadr x) a))))))
+
+; We are actually only interested in ADR lists whose lengths lie between 2 and
+; 5, and there are only a finite number of them.  Proofs are easier if we just
+; enumerate the cases.
+
+(defthm enumerate-dr-listps
+  (implies (and (dr-listp dr-list)
+;                (<= 2 (len dr-list)) ; !!!
+                (<= (len dr-list) 5))
+           (member dr-list
+                   '((#\R)
+                     (#\D #\R)
+                     (#\D #\D #\R)
+                     (#\D #\D #\D #\R)
+                     (#\D #\D #\D #\D #\R))))
+  :rule-classes nil)
+
+(defthm enumerate-adr-listps
+  (implies (and (adr-listp adr-list)
+;                (<= 2 (len adr-list)) ; !!!
+                (<= (len adr-list) 5))
+           (member adr-list
+                   '((#\R)
+                     (#\A #\R)
+                     (#\D #\R)
+                     (#\A #\D #\R)
+                     (#\D #\D #\R)
+                     (#\A #\D #\D #\R)
+                     (#\D #\D #\D #\R)
+                     (#\A #\D #\D #\D #\R)
+                     (#\D #\D #\D #\D #\R))))
+  :rule-classes nil)
+
+(in-theory (disable car-cdr-abbrev-name))
+
+(defun rev (x)
+  (if (endp x)
+      nil
+      (append (rev (cdr x)) (list (car x)))))
+
+(defthm evad-list-car-cdr-abbrev-name
+  (implies (and (adr-listp adr-list)
+                (<= 2 (len adr-list))
+                (<= (len adr-list) 5))
+           (equal (evad (list (car-cdr-abbrev-name adr-list) base) alist)
+                  (evad (compose-ad (rev adr-list) base) alist)))
+  :hints (("Goal" :use enumerate-adr-listps)))
+
+(defun equal-evad-compose-ad-hint (ad-list x y)
+  (cond ((endp ad-list) (list x y))
+        ((eql (car ad-list) #\A)
+         (equal-evad-compose-ad-hint (cdr ad-list) (list 'CAR x) (list 'CAR y)))
+        ((eql (car ad-list) #\D)
+         (equal-evad-compose-ad-hint (cdr ad-list) (list 'CDR x) (list 'CDR y)))
+        (t (equal-evad-compose-ad-hint (cdr ad-list) x y))))
+
+(defthm equal-evad-compose-ad
+  (implies (equal (evad x alist)
+                  (evad y alist))
+           (equal (equal (evad (compose-ad ad-list x) alist)
+                         (evad (compose-ad ad-list y) alist))
+                  t))
+  :hints (("Goal" :induct (equal-evad-compose-ad-hint ad-list x y))))
+
+
+; It would be nice if the above could be a congruence rule but unfortunately
+; the equivalence relation is not dyadic.
+
+(in-theory (disable mv-nth))
+
+(defthm compose-ac-append
+  (equal (compose-ad (append a b) base)
+         (compose-ad b (compose-ad a base))))
+
+
+
+;-----------------------------------------------------------------
+; The Proof
+
+(defthm make-reversed-ad-list-spec
+  (implies (ad-listp ans)
+           (and (implies ans (mv-nth 0 (make-reversed-ad-list term ans)))
+                (implies (not (mv-nth 0 (make-reversed-ad-list term ans)))
+                         (equal (mv-nth 1 (make-reversed-ad-list term ans)) term))
+                (ad-listp (mv-nth 0 (make-reversed-ad-list term ans)))
+                (equal (evad (compose-ad (mv-nth 0 (make-reversed-ad-list term ans))
+                                         (mv-nth 1 (make-reversed-ad-list term ans)))
+                             alist)
+                       (evad (compose-ad ans term) alist)))))
+
+; The inductive part of the proof that pretty-parse-ad-list is correct is for
+; the case when adr-list is actually just a dr-listp.  The case where adr-list
+; is an adr-listp is just a case split away.
+
+(defthm dr-listp-len-1-rev
+  (implies (and (dr-listp dr-list)
+                (equal (len dr-list) 1))
+           (equal (rev dr-list) '(#\R))))
+
+(defthm car-cdr-abbrev-name-adr-list-not-quote
+   (implies (and (adr-listp adr-list)
+;                 (<= 2 (len adr-list)) ; !!!
+                 (<= (len adr-list) 5))
+            (not (equal (car-cdr-abbrev-name adr-list) 'quote)))
+   :hints (("Goal" :use enumerate-adr-listps)))
+
+(defthm car-cdr-abbrev-name-dr-list-not-quote
+   (implies (and (dr-listp adr-list)
+;                 (<= 2 (len adr-list)) ; !!!
+                 (<= (len adr-list) 5))
+            (not (equal (car-cdr-abbrev-name adr-list) 'quote)))
+   :hints (("Goal" :use enumerate-dr-listps)))
+
+(defun evad-pretty-parse-ad-list-hint (ad-list dr-list n x y)
+  (declare (xargs :measure (llist (acl2-count ad-list) (nfix n))
+                  :well-founded-relation l<))
+  (cond
+   ((eql n 5)
+    (evad-pretty-parse-ad-list-hint
+     ad-list '(#\R)
+     1
+     (list (car-cdr-abbrev-name dr-list)
+           x)
+     (list (car-cdr-abbrev-name dr-list)
+           y)))
+   ((endp ad-list)
+    (list x y))
+   ((eql (car ad-list) #\A)
+    (evad-pretty-parse-ad-list-hint
+     (cdr ad-list)
+     '(#\R)
+     1
+     (list (car-cdr-abbrev-name (cons #\A dr-list))
+           x)
+     (list (car-cdr-abbrev-name (cons #\A dr-list))
+           y)))
+   (t (evad-pretty-parse-ad-list-hint
+       (cdr ad-list)
+       (cons #\D dr-list)
+       (+ 1 n)
+       x
+       y))))
+
+(defthm evad-pretty-parse-ad-list
+  (implies (and (equal (evad x alist)
+                       (evad y alist))
+                (ad-listp ad-list)
+                (dr-listp dr-list)
+                (equal (len dr-list) n)
+                (<= 1 n)
+                (<= n 5))
+           (equal (equal (evad (pretty-parse-ad-list ad-list dr-list n x) alist)
+                         (evad (pretty-parse-ad-list ad-list dr-list n y) alist))
+                  t))
+  :hints (("Goal" :induct (evad-pretty-parse-ad-list-hint ad-list dr-list n x y))
+          ("Subgoal *1/2'''" :in-theory (enable evad-constraint-0))
+          ("Subgoal *1/1''"  :in-theory (enable evad-constraint-0))))
+
+; By the way, evad-constraint-0, enabled above, allows us to evad (fn x ...)
+; for any fn other than QUOTE, expressing the answer in terms of the evads of
+; the x....
+
+(encapsulate
+ nil
+ (local (defun compose-d (lst base)
+          (cond ((endp lst) base)
+                ((eql (car lst) #\R) (compose-d (cdr lst) base))
+                (t (list 'cdr (compose-d (cdr lst) base))))))
+
+ (local
+  (defthm compose-d-lemma1
+    (implies (dr-listp dr-list)
+             (equal (compose-ad dr-list base)
+                    (compose-d dr-list base)))
+    :hints (("Goal" :induct (compose-ad dr-list base)))))
+
+ (local
+  (defthm compose-d-lemma2
+    (implies (dr-listp dr-list)
+             (equal (compose-ad (rev dr-list) base)
+                    (compose-d dr-list base)))))
+
+ (defthm rev-dr-list-is-no-op
+   (implies (dr-listp dr-list)
+            (equal (compose-ad (rev dr-list) base)
+                   (compose-ad dr-list base)))))
+
+(defthm pretty-parse-ad-list-spec
+  (implies (and (ad-listp ad-list)
+                (dr-listp dr-list)
+                (equal (len dr-list) n)
+                (<= 1 n)
+                (<= n 5))
+           (equal (evad (pretty-parse-ad-list ad-list dr-list n base) alist)
+                  (evad (compose-ad ad-list (compose-ad (rev dr-list) base)) alist)))
+  :hints (("Goal" :induct (pretty-parse-ad-list ad-list dr-list n base))
+          ("Subgoal *1/3'''" :use enumerate-dr-listps)
+          ("Subgoal *1/1" :use enumerate-dr-listps)))
+
+(defthm untranslate-car-cdr-nest-correct
+  (equal (evad term alist)
+         (evad (untranslate-car-cdr-nest term) alist))
+  :rule-classes nil)
